Generalize congruence-and-bound automation for ML-KEM
This extends GEN_CONGBOUND_RULE and CONGBOUND_RULE, which are used
in some ML-KEM proofs to propagate congruences and bounds, in
several ways:

 * Any specific word size are allowed for generic operations like
   word addition and subtraction

 * Word multiplication is also handled (with any specific size)

 * Sign-extension is handled (for any two specific sizes)

 * A standard Montgomery reduction sequence for ML-KEM is handled

arm/proofs/utils/mlkem.ml
@@ -139,7 +139,8 @@ let INVERSE_NTT_CONV =
   ONCE_DEPTH_CONV EXP_MOD_CONV THENC INT_REDUCE_CONV;;
 
 (* ------------------------------------------------------------------------- *)
-(* Abbreviate the Barrett reduction and multiplication patterns in the code. *)
+(* Abbreviate the Barrett reduction and multiplication and Montgomery        *)
+(* reduction patterns in the code.                                           *)
 (* ------------------------------------------------------------------------- *)
 
 let barred = define
@@ -158,53 +159,105 @@ let barmul = define
            (word_mul (iword_saturate((&2 * ival a * k + &32768) div &65536))
                      (word 3329))`;;
 
+let montred = define
+   `(montred:int32->int16) x =
+    word_subword
+     (word_add
+       (word_mul ((word_sx:int16->int32)
+                    (word_mul (word_subword x (0,16)) (word 3327)))
+                 (word 3329))
+       x)
+     (16,16)`;;
+
 (* ------------------------------------------------------------------------- *)
 (* Congruence-and-bound propagation, just recursion on the expression tree.  *)
 (* ------------------------------------------------------------------------- *)
 
 let CONGBOUND_ATOM = prove
- (`!x:int16. (ival x == ival x) (mod &3329) /\
-             -- &32768 <= ival x /\ ival x <= &32767`,
-  GEN_TAC THEN CONJ_TAC THENL [CONV_TAC INTEGER_RULE; BOUNDER_TAC[]]);;
+ (`!x:N word. (ival x == ival x) (mod &3329) /\
+              --(&2 pow (dimindex(:N) - 1)) <= ival x /\
+              ival x <= &2 pow (dimindex(:N) - 1) - &1`,
+  GEN_TAC THEN REWRITE_TAC[INT_ARITH `x:int <= y - &1 <=> x < y`] THEN
+  REWRITE_TAC[IVAL_BOUND] THEN INTEGER_TAC);;
 
 let CONGBOUND_ATOM_GEN = prove
- (`!x:int16. abs(ival x) <= n
-           ==> (ival x == ival x) (mod &3329) /\ --n <= ival x /\ ival x <= n`,
+ (`!x:N word. abs(ival x) <= n
+              ==> (ival x == ival x) (mod &3329) /\ --n <= ival x /\ ival x <= n`,
   REWRITE_TAC[INTEGER_RULE `(x:int == x) (mod n)`] THEN INT_ARITH_TAC);;
 
+let CONGBOUND_IWORD = prove
+ (`!x. ((x == x') (mod &3329) /\ l <= x /\ x <= u)
+       ==> --(&2 pow (dimindex(:N) - 1)) <= l /\ u <= &2 pow (dimindex(:N) - 1) - &1
+           ==> (ival(iword x:N word) == x') (mod &3329) /\
+               l <= ival(iword x:N word) /\ ival(iword x:N word) <= u`,
+  GEN_TAC THEN STRIP_TAC THEN STRIP_TAC THEN REWRITE_TAC[word_sx] THEN
+  W(MP_TAC o PART_MATCH (lhand o rand) IVAL_IWORD o lhand o rand o rand o snd) THEN
+  ANTS_TAC THENL [ASM_INT_ARITH_TAC; DISCH_THEN SUBST1_TAC] THEN
+  ASM_REWRITE_TAC[]);;
+
+let CONGBOUND_WORD_SX = prove
+ (`!x:M word.
+        ((ival x == x') (mod &3329) /\ l <= ival x /\ ival x <= u)
+        ==> --(&2 pow (dimindex(:N) - 1)) <= l /\ u <= &2 pow (dimindex(:N) - 1) - &1
+            ==> (ival(word_sx x:N word) == x') (mod &3329) /\
+                l <= ival(word_sx x:N word) /\ ival(word_sx x:N word) <= u`,
+  REWRITE_TAC[word_sx; CONGBOUND_IWORD]);;
+
 let CONGBOUND_WORD_ADD = prove
- (`!x y:int16.
+ (`!x y:N word.
         ((ival x == x') (mod &3329) /\ lx <= ival x /\ ival x <= ux) /\
         ((ival y == y') (mod &3329) /\ ly <= ival y /\ ival y <= uy)
-        ==> -- &32768 <= lx + ly /\ ux + uy <= &32767
+        ==> --(&2 pow (dimindex(:N) - 1)) <= lx + ly /\
+            ux + uy <= &2 pow (dimindex(:N) - 1) - &1
             ==> (ival(word_add x y) == x' + y') (mod &3329) /\
                 lx + ly <= ival(word_add x y) /\
                 ival(word_add x y) <= ux + uy`,
-  REPEAT GEN_TAC THEN STRIP_TAC THEN STRIP_TAC THEN
-  SUBGOAL_THEN `ival(word_add x y:int16) = ival x + ival y` SUBST_ALL_TAC THENL
-   [MATCH_MP_TAC INT_CONG_IMP_EQ THEN
-    EXISTS_TAC `(&2:int) pow dimindex(:16)` THEN
-    REWRITE_TAC[ICONG_WORD_ADD] THEN
-    MP_TAC(ISPEC `word_add x y:int16` IVAL_BOUND) THEN
-    REWRITE_TAC[DIMINDEX_16; ARITH] THEN ASM_INT_ARITH_TAC;
-    ASM_SIMP_TAC[INT_CONG_ADD] THEN ASM_INT_ARITH_TAC]);;
+  REPEAT GEN_TAC THEN REWRITE_TAC[WORD_ADD_IMODULAR; imodular] THEN
+  STRIP_TAC THEN STRIP_TAC THEN
+  MATCH_MP_TAC(REWRITE_RULE[IMP_IMP] CONGBOUND_IWORD) THEN
+  ASM_SIMP_TAC[INT_CONG_ADD] THEN ASM_INT_ARITH_TAC);;
 
 let CONGBOUND_WORD_SUB = prove
- (`!x y:int16.
+ (`!x y:N word.
         ((ival x == x') (mod &3329) /\ lx <= ival x /\ ival x <= ux) /\
         ((ival y == y') (mod &3329) /\ ly <= ival y /\ ival y <= uy)
-        ==> -- &32768 <= lx - uy /\ ux - ly <= &32767
+        ==> --(&2 pow (dimindex(:N) - 1)) <= lx - uy /\
+            ux - ly <= &2 pow (dimindex(:N) - 1) - &1
             ==> (ival(word_sub x y) == x' - y') (mod &3329) /\
                 lx - uy <= ival(word_sub x y) /\
                 ival(word_sub x y) <= ux - ly`,
-  REPEAT GEN_TAC THEN STRIP_TAC THEN STRIP_TAC THEN
-  SUBGOAL_THEN `ival(word_sub x y:int16) = ival x - ival y` SUBST_ALL_TAC THENL
-   [MATCH_MP_TAC INT_CONG_IMP_EQ THEN
-    EXISTS_TAC `(&2:int) pow dimindex(:16)` THEN
-    REWRITE_TAC[ICONG_WORD_SUB] THEN
-    MP_TAC(ISPEC `word_sub x y:int16` IVAL_BOUND) THEN
-    REWRITE_TAC[DIMINDEX_16; ARITH] THEN ASM_INT_ARITH_TAC;
-    ASM_SIMP_TAC[INT_CONG_SUB] THEN ASM_INT_ARITH_TAC]);;
+  REPEAT GEN_TAC THEN REWRITE_TAC[WORD_SUB_IMODULAR; imodular] THEN
+  STRIP_TAC THEN STRIP_TAC THEN
+  MATCH_MP_TAC(REWRITE_RULE[IMP_IMP] CONGBOUND_IWORD) THEN
+  ASM_SIMP_TAC[INT_CONG_SUB] THEN ASM_INT_ARITH_TAC);;
+
+let CONGBOUND_WORD_MUL = prove
+ (`!x y:N word.
+        ((ival x == x') (mod &3329) /\ lx <= ival x /\ ival x <= ux) /\
+        ((ival y == y') (mod &3329) /\ ly <= ival y /\ ival y <= uy)
+        ==> --(&2 pow (dimindex(:N) - 1))
+            <= min (lx * ly) (min (lx * uy) (min (ux * ly) (ux * uy))) /\
+            max (lx * ly) (max (lx * uy) (max (ux * ly) (ux * uy)))
+            <= &2 pow (dimindex(:N) - 1) - &1
+            ==> (ival(word_mul x y) == x' * y') (mod &3329) /\
+                min (lx * ly) (min (lx * uy) (min (ux * ly) (ux * uy)))
+                <= ival(word_mul x y) /\
+                ival(word_mul x y)
+                <= max (lx * ly) (max (lx * uy) (max (ux * ly) (ux * uy)))`,
+  let lemma = prove
+     (`l:int <= x /\ x <= u
+       ==> !a. a * l <= a * x /\ a * x <= a * u \/
+               a * u <= a * x /\ a * x <= a * l`,
+      MESON_TAC[INT_LE_NEGTOTAL; INT_LE_LMUL;
+                INT_ARITH `a * x:int <= a * y <=> --a * y <= --a * x`]) in
+  REPEAT GEN_TAC THEN
+  DISCH_THEN(CONJUNCTS_THEN(CONJUNCTS_THEN2 ASSUME_TAC MP_TAC)) THEN
+  DISCH_THEN(ASSUME_TAC o SPEC `ival(x:N word)` o MATCH_MP lemma) THEN
+  DISCH_THEN(MP_TAC o MATCH_MP lemma) THEN DISCH_THEN(fun th ->
+        ASSUME_TAC(SPEC `ly:int` th) THEN ASSUME_TAC(SPEC `uy:int` th)) THEN
+  REWRITE_TAC[WORD_MUL_IMODULAR; imodular] THEN STRIP_TAC THEN
+  MATCH_MP_TAC(REWRITE_RULE[IMP_IMP] CONGBOUND_IWORD) THEN
+  ASM_SIMP_TAC[INT_CONG_MUL] THEN ASM_INT_ARITH_TAC);;
 
 let CONGBOUND_BARRED = prove
  (`!a a' l u.
@@ -293,39 +346,112 @@ let CONGBOUND_BARMUL = prove
    `l:int <= x /\ x <= u ==> abs x <= max (abs l) (abs u)`] THEN
   CONV_TAC INT_ARITH);;
 
+let MONTRED_LEMMA = prove
+ (`!x. &2 pow 16 * ival(montred x) =
+       ival(word_add
+         (word_mul (word_sx(iword(ival x * &3327):int16)) (word 3329)) x)`,
+  GEN_TAC THEN REWRITE_TAC[montred] THEN REWRITE_TAC[WORD_BLAST
+   `word_subword (x:int32) (0,16):int16 = word_sx x`] THEN
+  REWRITE_TAC[IWORD_INT_MUL; GSYM word_sx; GSYM WORD_IWORD] THEN
+  REWRITE_TAC[WORD_BLAST `(word_sx:int32->int16) x = word_zx x`] THEN
+  CONV_TAC INT_REDUCE_CONV THEN MATCH_MP_TAC(BITBLAST_RULE
+   `word_and x (word 65535):int32 = word 0
+    ==> &65536 * ival(word_subword x (16,16):int16) = ival x`) THEN
+  REWRITE_TAC[BITBLAST_RULE
+   `word_and x (word 65535):int32 = word 0 <=> word_zx x:int16 = word 0`] THEN
+  W(MP_TAC o PART_MATCH (lhand o rand) WORD_ZX_ADD o lhand o snd) THEN
+  REWRITE_TAC[DIMINDEX_16; DIMINDEX_32; ARITH] THEN DISCH_THEN SUBST1_TAC THEN
+  W(MP_TAC o PART_MATCH (lhand o rand) WORD_ZX_MUL o lhand o lhand o snd) THEN
+  REWRITE_TAC[DIMINDEX_16; DIMINDEX_32; ARITH] THEN DISCH_THEN SUBST1_TAC THEN
+  REWRITE_TAC[WORD_BLAST `word_zx(word_sx (x:int16):int32) = x`] THEN
+  REWRITE_TAC[GSYM VAL_EQ_0; VAL_WORD_ADD; VAL_WORD_MUL; VAL_WORD] THEN
+  CONV_TAC MOD_DOWN_CONV THEN REWRITE_TAC[GSYM DIVIDES_MOD; DIMINDEX_16] THEN
+  CONV_TAC WORD_REDUCE_CONV THEN MATCH_MP_TAC(NUMBER_RULE
+   `(a * b + 1 == 0) (mod d) ==> d divides ((x * a) * b + x)`) THEN
+  REWRITE_TAC[CONG] THEN ARITH_TAC);;
+
+let CONGBOUND_MONTRED = prove
+ (`!a a' l u.
+      (ival a == a') (mod &3329) /\ l <= ival a /\ ival a <= u
+      ==> --(&2038398976) <= l /\ u <= &2038402304
+          ==> (ival(montred a) == &(inverse_mod 3329 65536) * a') (mod &3329) /\
+              (l - &109084672) div &2 pow 16 <= ival(montred a) /\
+              ival(montred a) <= &1 + (u + &109081343) div &2 pow 16`,
+  REPEAT GEN_TAC THEN STRIP_TAC THEN STRIP_TAC THEN
+  CONV_TAC NUM_REDUCE_CONV THEN CONV_TAC(ONCE_DEPTH_CONV INVERSE_MOD_CONV) THEN
+  MP_TAC(SPECL [`&169:int`; `(&2:int) pow 16`; `&3329:int`] (INTEGER_RULE
+ `!d e n:int. (e * d == &1) (mod n)
+              ==> !x y. ((x == d * y) (mod n) <=> (e * x == y) (mod n))`)) THEN
+  ANTS_TAC THENL
+   [REWRITE_TAC[GSYM INT_REM_EQ] THEN INT_ARITH_TAC;
+    DISCH_THEN(fun th -> REWRITE_TAC[th])] THEN
+  ONCE_REWRITE_TAC[INT_ARITH
+   `l:int <= x <=> &2 pow 16 * l <= &2 pow 16 * x`] THEN
+  REWRITE_TAC[MONTRED_LEMMA] THEN
+  REWRITE_TAC[WORD_RULE
+   `word_add (word_mul a b) c = iword(ival a * ival b + ival c)`] THEN
+  ASM_SIMP_TAC[IVAL_WORD_SX; DIMINDEX_16; DIMINDEX_32; ARITH] THEN
+  W(MP_TAC o PART_MATCH (lhand o rand) IVAL_IWORD o
+   lhand o rator o lhand o snd) THEN
+  REWRITE_TAC[DIMINDEX_32] THEN CONV_TAC(DEPTH_CONV WORD_NUM_RED_CONV) THEN
+  W(MP_TAC o C ISPEC IVAL_BOUND o
+    rand o funpow 3 lhand o rand o lhand o lhand o snd) THEN
+  REWRITE_TAC[DIMINDEX_16; ARITH] THEN STRIP_TAC THEN
+  ANTS_TAC THENL [ASM_INT_ARITH_TAC; DISCH_THEN SUBST1_TAC] THEN
+  ASM_REWRITE_TAC[INTEGER_RULE
+   `(a * p + x:int == y) (mod p) <=> (x == y) (mod p)`] THEN
+  ASM_INT_ARITH_TAC);;
+
+let DIMINDEX_INT_REDUCE_CONV =
+  DEPTH_CONV(WORD_NUM_RED_CONV ORELSEC DIMINDEX_CONV) THENC
+  INT_REDUCE_CONV;;
+
+let CONCL_BOUNDS_RULE =
+  CONV_RULE(BINOP2_CONV
+          (LAND_CONV(RAND_CONV DIMINDEX_INT_REDUCE_CONV))
+          (BINOP2_CONV
+           (LAND_CONV DIMINDEX_INT_REDUCE_CONV)
+           (RAND_CONV DIMINDEX_INT_REDUCE_CONV)));;
+
+let SIDE_ELIM_RULE th =
+  MP th (EQT_ELIM(DIMINDEX_INT_REDUCE_CONV(lhand(concl th))));;
+
 let rec GEN_CONGBOUND_RULE aboths tm =
   match tm with
     Comb(Comb(Const("barmul",_),kb),t) ->
         let ktm,btm = dest_pair kb and th0 = GEN_CONGBOUND_RULE aboths t in
         let th1 = SPECL [ktm;btm] (MATCH_MP CONGBOUND_BARMUL th0) in
-        let th2 = DEPTH_CONV WORD_NUM_RED_CONV (lhand(concl th1)) in
-        let th3 = MP th1 (EQT_ELIM th2) in
-        CONV_RULE(BINOP2_CONV
-          (LAND_CONV(RAND_CONV(DEPTH_CONV WORD_NUM_RED_CONV)))
-          (BINOP2_CONV
-           (LAND_CONV(DEPTH_CONV WORD_NUM_RED_CONV))
-           (RAND_CONV(DEPTH_CONV WORD_NUM_RED_CONV)))) th3
+        CONCL_BOUNDS_RULE(SIDE_ELIM_RULE th1)
   | Comb(Const("barred",_),t) ->
         let th1 = GEN_CONGBOUND_RULE aboths t in
         MATCH_MP CONGBOUND_BARRED th1
+  | Comb(Const("montred",_),t) ->
+        let th1 = GEN_CONGBOUND_RULE aboths t in
+        CONCL_BOUNDS_RULE(SIDE_ELIM_RULE(MATCH_MP CONGBOUND_MONTRED th1))
+  | Comb(Const("word_sx",_),t) ->
+        let th0 = GEN_CONGBOUND_RULE aboths t in
+        let tyin = type_match
+         (type_of(rator(rand(lhand(funpow 4 rand (snd(dest_forall
+            (concl CONGBOUND_WORD_SX)))))))) (type_of(rator tm)) [] in
+        let th1 = MATCH_MP (INST_TYPE tyin CONGBOUND_WORD_SX) th0 in
+        CONCL_BOUNDS_RULE(SIDE_ELIM_RULE th1)
   | Comb(Comb(Const("word_add",_),ltm),rtm) ->
         let lth = GEN_CONGBOUND_RULE aboths ltm
         and rth = GEN_CONGBOUND_RULE aboths rtm in
         let th1 = MATCH_MP CONGBOUND_WORD_ADD (CONJ lth rth) in
-        let th2 = DEPTH_CONV WORD_NUM_RED_CONV (lhand(concl th1)) in
-        let th3 = MP th1 (EQT_ELIM th2) in
-        CONV_RULE(RAND_CONV (BINOP2_CONV
-           (LAND_CONV INT_ADD_CONV) (RAND_CONV INT_ADD_CONV))) th3
+        CONCL_BOUNDS_RULE(SIDE_ELIM_RULE th1)
   | Comb(Comb(Const("word_sub",_),ltm),rtm) ->
         let lth = GEN_CONGBOUND_RULE aboths ltm
         and rth = GEN_CONGBOUND_RULE aboths rtm in
         let th1 = MATCH_MP CONGBOUND_WORD_SUB (CONJ lth rth) in
-        let th2 = DEPTH_CONV WORD_NUM_RED_CONV (lhand(concl th1)) in
-        let th3 = MP th1 (EQT_ELIM th2) in
-        CONV_RULE(RAND_CONV (BINOP2_CONV
-           (LAND_CONV INT_SUB_CONV) (RAND_CONV INT_SUB_CONV))) th3
+        CONCL_BOUNDS_RULE(SIDE_ELIM_RULE th1)
+  | Comb(Comb(Const("word_mul",_),ltm),rtm) ->
+        let lth = GEN_CONGBOUND_RULE aboths ltm
+        and rth = GEN_CONGBOUND_RULE aboths rtm in
+        let th1 = MATCH_MP CONGBOUND_WORD_MUL (CONJ lth rth) in
+        CONCL_BOUNDS_RULE(SIDE_ELIM_RULE th1)
   | _ -> (try MATCH_MP CONGBOUND_ATOM_GEN
                (find ((=) tm o rand o rand o lhand o concl) aboths)
-          with Failure _ -> ISPEC tm CONGBOUND_ATOM);;
+          with Failure _ -> CONCL_BOUNDS_RULE(ISPEC tm CONGBOUND_ATOM));;
 
 let CONGBOUND_RULE = GEN_CONGBOUND_RULE [];;
